Change type of ghost state to an hlist
Semantics now enforces that ghost state is actually an hlist (with type
indices as Types rather than Sets, as in the memory), since the
modularity story is the same for memory and ghost state.

src/Bank.v
@@ -21,7 +21,8 @@ Section Bank.
   | from1 : forall (amount:nat), ledger_entry
   | from2 : forall (amount:nat), ledger_entry.
 
-  Definition State := list ledger_entry.
+  Definition Scontents : list Type := [(list ledger_entry):Type].
+  Definition Ledger : svar Scontents _ := HFirst.
 
   (* the memory for a bank is empty *)
   Definition Mcontents := @nil Set.
@@ -34,7 +35,7 @@ Section Bank.
                      end
     end.
 
-  Fixpoint balances' (entries:State) accum : (nat * nat) :=
+  Fixpoint balances' (entries:list ledger_entry) accum : (nat * nat) :=
     match entries with
     | nil => accum
     | entry :: xs => balances' xs (add_entry accum entry)
@@ -42,30 +43,32 @@ Section Bank.
 
   Definition balances entries := balances' entries (100, 0).
 
-  Definition bankR (_:ID) : Relation State :=
-    fun ledger ledger' =>
+  Definition bankR (_:ID) : Relation Scontents :=
+    fun s s' =>
+    let ledger := get Ledger s in
+    let ledger' := get Ledger s' in
     ledger' = ledger \/
     exists entry, ledger' = ledger ++ [entry].
 
-  Definition bankI ledger bal1 bal2 :=
-    balances ledger = (bal1, bal2).
+  Definition bankI (s:S Scontents) bal1 bal2 :=
+    balances (get Ledger s) = (bal1, bal2).
 
-  Definition bankPred (_:M Mcontents) ledger : DISK_PRED :=
+  Definition bankPred (_:M Mcontents) s : DISK_PRED :=
     fun d =>
       exists bal1 bal2,
         #bal1 + #bal2 = 100 /\
         exists F rest1 rest2 ,
           d |= F * rep rest1 rest2 bal1 bal2 /\
-          bankI ledger #bal1 #bal2.
+          bankI s #bal1 #bal2.
 
-  Definition bankLockR : ID -> Relation State := fun _ _ _ => True.
+  Definition bankLockR : ID -> Relation Scontents := fun _ _ _ => True.
 
-  Definition bankLockI : Invariant Mcontents State := fun _ _ _ => True.
+  Definition bankLockI : Invariant Mcontents Scontents := fun _ _ _ => True.
 
-  Definition bankS : transitions Mcontents State :=
+  Definition bankS : transitions Mcontents Scontents :=
     Build_transitions bankR bankLockR bankPred bankLockI.
 
-  Local Hint Unfold rep State bankR bankLockR bankI bankLockI : prog.
+  Local Hint Unfold rep bankR bankLockR bankI bankLockI : prog.
 
   Definition transfer {T S} amount rx : prog Mcontents S T :=
     bal1 <- Read acct1;
@@ -75,7 +78,10 @@ Section Bank.
     rx tt.
 
   (* an update function that adds an entry to the ledger for transfer *)
-  Definition record_transfer amount ledger : State := ledger ++ [from1 amount].
+  Definition record_transfer amount (s:S Scontents) :=
+    Eval cbn in
+    let ledger := get Ledger s in
+    set Ledger (ledger ++ [from1 amount]) s.
 
   Hint Unfold record_transfer : prog.
 
@@ -166,16 +172,21 @@ Section Bank.
 
   Hint Resolve record_correct.
 
-  Lemma star_bankR : forall tid ledger ledger',
-      star (othersR bankR tid) ledger ledger' ->
+  Lemma star_bankR : forall tid s s',
+      star (othersR bankR tid) s s' ->
+      let ledger := get Ledger s in
+      let ledger' := get Ledger s' in
       exists ledger_ext, ledger' = ledger ++ ledger_ext.
   Proof.
     unfold othersR, bankR.
     induction 1.
     exists nil; rewrite app_nil_r; auto.
 
-    intuition; repeat deex; eauto.
-    eexists.
+    intuition; repeat deex;
+      repeat match goal with
+      | [ H: get Ledger _ = _ |- _ ] =>
+        rewrite H in *
+      end; eauto.
     rewrite <- app_assoc.
     eauto.
   Qed.
@@ -219,13 +230,14 @@ Section Bank.
   Lemma bank_invariant_transfer : forall F s m rest1 rest2 bal1 bal2 amount,
       #bal1 + #bal2 = 100 ->
       #bal1 >= amount ->
-      balances s = (#bal1, #bal2) ->
+      balances (get Ledger s) = (#bal1, #bal2) ->
       (acct2 |-> (Valuset (bal2 ^+ $ amount) rest2) *
        acct1 |-> (Valuset (bal1 ^- $ amount) rest1) * F) =p=>
-  bankPred m (s ++ [from1 amount]).
+  bankPred m (set Ledger (get Ledger s ++ [from1 amount]) s).
   Proof.
     unfold bankPred, pimpl, pred_in; intros.
     repeat (autounfold with prog).
+    simpl_get_set.
     exists (bal1 ^- ($ amount)).
     exists (bal2 ^+ ($ amount)).
     repeat eexists; eauto.
@@ -242,24 +254,30 @@ Section Bank.
   Theorem transfer_yield_ok : forall rest1 rest2 bal1 bal2 amount,
     bankS TID: tid |-
     {{ F,
-     | PRE d m l0 l: d |= F * rep rest1 rest2 bal1 bal2 /\
+     | PRE d m s0 s: d |= F * rep rest1 rest2 bal1 bal2 /\
                      #bal1 + #bal2 = 100 /\
                      #bal1 >= amount /\
-                     bankI l #bal1 #bal2 /\
-                     l0 = l
-     | POST d' m' l0' l' _: d' |= bankPred m' l' /\
+                     bankI s #bal1 #bal2 /\
+                     s0 = s
+     | POST d' m' s0' s' _: d' |= bankPred m' s' /\
+                            let l := get Ledger s in
+                            let l' := get Ledger s' in
                             firstn (length l + 1) l' = l ++ [from1 amount] /\
-                            l0' = l'
+                            s0' = s'
      | CRASH d'c : True
     }} transfer_yield amount.
   Proof.
-    hoare.
+    hoare pre (step_simplifier; simpl_get_set).
     pred_apply; cancel; eauto.
 
     match goal with
     | [ H: star _ _ _ |- _ ] => apply star_bankR in H; auto
     end.
-    deex; subst.
+    deex.
+    match goal with
+    | [ H: get Ledger _ = _ |- _ ] =>
+      rewrite H; simpl_get_set
+    end.
     apply firstn_length_app.
     rewrite app_length; auto.
   Qed.
