src/Locking.v
@@ -1,14 +1,11 @@
 Require Import EventCSL.
-Require Import Hlist.
 
 Set Implicit Arguments.
 
 Section Locking.
 
 Variable Mcontents : list Set.
-Variable Scontents : list Set.
-
-Notation S := (hlist (fun T:Set => T) Scontents).
+Variable Scontents : list Type.
 
 Inductive MutexOwner : Set :=
 | NoOwner
@@ -16,8 +13,8 @@ Inductive MutexOwner : Set :=
 
 (** given a lock variable and some other variable v, generate a
 relation for tid that makes the variable read-only for non-owners. *)
-Definition lock_protects (lvar : var Scontents MutexOwner)
-           {tv} (v : var Scontents tv) tid (s s': S) :=
+Definition lock_protects (lvar : svar Scontents MutexOwner)
+           {tv} (v : svar Scontents tv) tid (s s': S Scontents) :=
   forall owner_tid,
     get lvar s = Owned owner_tid ->
     tid <> owner_tid ->
@@ -25,7 +22,8 @@ Definition lock_protects (lvar : var Scontents MutexOwner)
 
 Hint Unfold lock_protects : prog.
 
-Inductive lock_protocol (lvar : var Scontents MutexOwner) (tid : ID) : S -> S -> Prop :=
+Inductive lock_protocol (lvar : svar Scontents MutexOwner) (tid : ID) :
+  S Scontents -> S Scontents -> Prop :=
 | NoChange : forall s s', get lvar s  = get lvar s' ->
                      lock_protocol lvar tid s s'
 | OwnerRelease : forall s s', get lvar s = Owned tid ->
@@ -39,8 +37,8 @@ Hint Constructors lock_protocol.
 
 Inductive ghost_lock_invariant
           (lvar : var Mcontents Mutex)
-          (glvar : var Scontents MutexOwner)
-          (m : M Mcontents) (s : S) : Prop :=
+          (glvar : svar Scontents MutexOwner)
+          (m : M Mcontents) (s : S Scontents) : Prop :=
 | LockOpen : get lvar m = Open -> get glvar s = NoOwner ->
              ghost_lock_invariant lvar glvar m s
 | LockOwned : forall tid, get lvar m = Locked -> get glvar s = Owned tid ->
